## Question 1

a)

$$
\begin{align*}
\vec{r} &= 2i -3j + k +i - 2j - k + 2i + 3j \\
        &= 5i -2j \\
\\
\vec{s} &= 4i - 6j + 2k - i + 2j + k + 6i + 9j \\
        &= 9i + 5j + 3k
\end{align*}
$$

b)

$$
\begin{align*}
\vec{u} \cdot \vec{v} = (2i - 3j + k) \cdot (i - 2j - k) = 2 + 6 - 1 = 7
\end{align*}
$$

c)

$$
\begin{align*}
2\vec{u} - \vec{w} &= 2i - 9j + 2k \\
\\
2\vec{u} + 2\vec{w} &= 2(\vec{u} + \vec{w}) = 8i + 2k
\end{align*}
$$

$$
(2\vec{u} - \vec{w}) \times (2\vec{u} + 2\vec{w}) = \begin{vmatrix}
i & j & k \\
2 & -9 & 2 \\
8 & 0 & 2 \\
\end{vmatrix}
= -18i + 12j + 72k
$$

d) 

We will show two approaches to find $\vec{a}$, which we will later normalize by $\frac{1}{||\vec{a}||}$.

**Approch one:** Using cross product.

By definition $\vec{a} = \vec{u} \times \vec{w}$. Calculating yields

$$
\vec{a} = \begin{vmatrix}
i & j & k \\
2 & -3 & 1 \\
2 & 3 & 0
\end{vmatrix} = -3i + 2j + 12k
$$

**Approach two:** Using the scalar product.

We know that $\vec{a} = (a_1, a_2, a_3)$ should satisfy $\vec{a} \cdot u = \vec{a} \cdot w = 0$. Therefore, we can write a system of equations:

$$
\begin{align*}
& 2a_1 - 3a_2 + a_3 = 0 \\
& 2a_1 + 3a_2 = 0 \\
\end{align*}
$$

From the second equation we get that $2a_1 = -3a_2$. Substituting in the first equation we get
$$
a_3 = 6a_2
$$

We have one degree of freedom. Set $a_2 = 2$ and get $\vec{a} = (-3, 2, 12)$ which is indeed a normal to $Span\{u, w\}$.

**Normalization**

From the above, we get that $\hat{a} = \frac{1}{||\vec{a}||} \vec{a} = \frac{1}{\sqrt{157}} (-3, 2, 12) = (-0.23, 0.15, 0.95)$

e)
$$
\begin{align}
(\vec{u}\cdot\vec{w})\vec{v} - (\vec{u}\cdot{\vec{v}})\vec{w}
&= 7\vec{v} - 7\vec{w} = 7(\vec{v} - \vec{w}) \\
&= (-7, -35, -7)
\end{align}
$$

f)

$$
\vec{u} \times \vec{v} = \begin{vmatrix}
i & j & k \\
2 & -3 & 1 \\
1 & -2 & -1
\end{vmatrix} = 3i + 3j - k
$$

$$
(\vec{u} \times \vec{v}) \cdot \vec{w} = (3i + 3j - k) \cdot (2i + 3j) = 14
$$