## Question 4

a)

On the x-axis:

$$
\sum F_x = 0 = m\vec{a}_x(t)
$$

therefore 
$$
\begin{align*}
\vec{a}_x(t) &= 0 \\
\vec{v}_x(t) &= v_0 \cos \theta \\
\vec{r}_x(t) &= v_0 t \cos \theta
\end{align*}
$$

On the y-axis:
$$
\sum F_y = -mg = m\vec{a}_y(t)
$$

therefore
$$
\begin{align*}
\vec{a}_y(t) &= -g \\
\vec{v}_y(t) &= v_0 \sin \theta - gt \\
\vec{r}_y(t) &= v_0 t \sin \theta - \frac{1}{2}gt^2
\end{align*}
$$

Finally
$$
\vec{r}(t) = (v_0 t \cos \theta) \hat{x} + (v_0 t \sin \theta - \frac{1}{2}gt^2) \hat{y}
$$

b)

$$
\begin{align*}
\vec{v}(t) &= (v_0 \cos \theta) \hat{x} + (v_0 \sin \theta - gt) \hat{y} \\
\vec{a}(t) &= -g \hat{y}
\end{align*}
$$

c)

$$
\theta = \cos^{-1} \frac{\vec{v} \cdot \vec{a}}{|\vec{a}| |\vec{v}|} = ... = \frac{gt - v_0 \sin \theta}{\sqrt{
    v_0^2 - 2v_0gt\sin \theta + (gt)^2
}}
$$