## Question 5

a)


We will denote $y$ as the axis perpendicular to the slope and $x$ as the axis parallel to the slope.

**State 1:** Mass is moving positively and decelerating.

The forces applied on the body:

- Downward gravitational force $mg\hat{j}$ which is decomposed to components $- mg sin (\theta) \hat{x}$ and $- mgcos(\theta)\hat{y}$ (remember, $x$ and $y$ are relative to the slope.)

- Normal force applied as opposition from the slope $N \hat{y}$.

- Friction force $- f_k \hat{x} = - \mu N \hat{x}$

Acceleration along the $y$ is 0, therefore
$$
\sum \vec{F_y} = 0 = N - mg\cos\theta \Rightarrow N = mg\cos\theta
$$

Denote by $a$ acceleration along the $x$ axis. We get that
$$
\sum \vec{F_x} = ma = -f_k - mg \sin \theta = - \mu mg\cos\theta - mg \sin \theta
$$

Denote $A = g \mu \cos \theta + g \sin \theta$ and we get that
$$
a = -A
$$

By integration,
$$
\begin{align*}
v(t) &= v_0 - At \\
r(t) &= v_0t - \frac{A}{2}t^2 \\
\end{align*}
$$

where we assigned $r(0) = 0$.

The mass will stop when the velocity is zero, i.e. $v(t) = 0$ which is when $t = t_1 = \frac{v_0}{A}$ (other than $t=0$). It's position will be
$$
r_1 = r(\frac{v_0}{A}) = \frac{v_0^2}{2A}
$$

**State 2:** Mass is sliding down the slope and accelerating negatively.

Forces applied here are the same, with the exception of the friction force which is now directed at the positive $x$ direction.

Again,
$$
\sum F_y = 0 = N - mg\cos\theta \Rightarrow N = mg\cos\theta
$$

$$
\sum F_x = ma = f_k - mg \sin \theta = \mu mg\cos\theta - mg \sin \theta
$$

Denote $B = \mu g \cos \theta - g \sin \theta$ and get that
$$
a = B
$$

By integration,
$$
\begin{align*}
v(t) &= Bt \\
r(t) &= \frac{B}{2}t^2 + r_1 = \frac{B}{2}t^2 + \frac{v_0^2}{2A}
\end{align*}
$$

where the initial velocity is 0 because the mass is still.

The mass will reach $r(t) = 0$  when $t^2 = - \frac{v_0^2}{AB}$, i.e. $t = t_2 = v_0 \sqrt{\frac{-1}{AB}}$.

**Conclusion**

The total time in which the mass will get back to its initial place is
$$
t_1 + t_2 = \frac{v_0}{A} + \sqrt{\frac{-v_0^2}{AB}} = \frac{v_0}{g \mu \cos \theta + g \sin \theta} + \sqrt{\frac{v_0^2}{(g \mu \cos \theta + g \sin \theta)(g \sin \theta - \mu g \cos \theta)}}
$$

b)

The final velocity is (according to the notations of the second state)
$$
v(t_2) = v_2 = B v_0 \sqrt{\frac{-1}{AB}} = v_0 \sqrt{\frac{-B}{A}}
$$

Therefore, the ratio $\frac{v_2}{v_0}$ is $\sqrt{\frac{-B}{A}} = \sqrt{\frac{g \sin \theta - \mu g \cos \theta}{g \mu \cos \theta + g \sin \theta}}$.