## Question 7

a)

Newton's second law gives:
$$
F = m \dot{v} = - k \sqrt{v}
$$

Thus 
$$
\dot{v} = - \frac{k}{m}\sqrt{v}
$$

b)

Using seperation of variables
$$
\int v^{-\frac{1}{2}} dv = - \frac{k}{m} \int dt
$$

$$
2 v ^{\frac{1}{2}} = -\frac{k}{m}t + C_0
$$

$$
v = \frac{(C_0 - \frac{k}{m}t)^2}{4}
$$

$$
v_0 = v(0) = \frac{C_0^2}{4} \Rightarrow C_0 = 2\sqrt{v_0}
$$

Finally
$$
v = \frac{(2\sqrt{v_0} - \frac{k}{m}t)^2}{4}
$$

c)

$$
r = \int v dt = \frac{1}{4} \int 4v_0 - 4 \frac{k \sqrt{v_0}}{m}t + (\frac{k}{m}t)^2 dt = \frac{1}{4}(4v_0 t - 2 \frac{k\sqrt{v_0}}{m}t^2) + \frac{k}{3m}t^3 + C_1)
$$

We know that $r(0) = 0$ so
$$
\frac{C_1}{4} = 0 \Rightarrow C_1 = 0
$$

Finally
$$
r = \frac{\frac{k}{3m}t^3 - 2 \frac{k\sqrt{v_0}}{m}t^2 + 4v_0 t}{4}
$$