
Denote

- $X \in \mathbb{F}^{3 \times 3} = (x_{i, j})$
- $K \in \mathbb{F}^{2 \times 1} = (k_{i, j})$

and $Y \in \mathbb{F}^{2 \times 3} = (y_{i, j})$ given by

$$
    X \ast K = Y
$$

Forall $r = 1, 2$ and $s = 1, 2, 3$ we calculate $y_{rs}$ b

$$
\begin{equation}
    y_{r, s} = x_{r, s} k_{1, 1} + x_{r+1, s} k_{2, 1}
\end{equation}
$$

Forall $i = 1, 2$, by the chain rule and (1) we get that

$$
    \frac{ \partial C }{ \partial k_{i, 1}} = \
    \sum_{r, s}\frac{ \partial C }{ \partial y_{r, s}} \frac{ \partial y_{r, s} }{ k_{i, 1 }} =\
    \sum_{r, s} \frac{ \partial C }{ \partial y_{r, s} } x_{r + i-1, s}
$$

Now we will notice that in (1), the derivative
${\frac{\partial y_{r, s}}{\partial x_{i,j}}}$
is non zero only when $j = s$ and $i \in \{ r, r+1\}$ (or the derivative itself result in 0). Therfore we get the followings:

Forall $i = 1$ and $j = 1, 2, 3$, by the chain rule and (1) we get that

$$
    \frac{ \partial C }{ \partial x_{i, j}} = \
    \sum_{r, s}\frac{ \partial C }{ \partial y_{r, s}} \frac{ \partial y_{r, s} }{ x_{i, j }} =\
    \frac {\partial C}{\partial y_{i, j}} k_{1, 1}
$$

Forall $i = 2, 3$ and $j = 1, 2, 3$, by the chain rule and (1) we get that

$$
    \frac{ \partial C }{ \partial x_{i, j}} = \
    \sum_{r, s}\frac{ \partial C }{ \partial y_{r, s}} \frac{ \partial y_{r, s} }{ x_{i, j }} =\
    \frac {\partial C}{\partial y_{i, j}} k_{1, 1} + \frac {\partial C}{\partial y_{i-1, j}} k_{2, 1}
$$

<!-- 
$$
    X \ast K = Y
$$



As

$$
\begin{bmatrix}
    x_{11} & x_{12} & x_{13} \\
    x_{21} & x_{22} & x_{23} \\
    x_{31} & x_{32} & x_{33} \\
\end{bmatrix}
\ast
\begin{bmatrix}
    k_{11} \\
    k_{21} \\
\end{bmatrix}
=
\begin{bmatrix}
    y_{11} & y_{12} & y_{13} \\
    y_{21} & y_{22} & y_{23} \\
\end{bmatrix}
$$

Thus, we can compute $Y$ by

$$
Y = \begin{bmatrix}
    x_{11} k_{11} + x_{21} k_{21} & x_{12} k_{11} + x_{22} k_{21} & x_{13} k_{11} + x_{23} k_{21} \\
    x_{21} k_{11} + x_{31} k_{21} & x_{22} k_{11} + x_{32} k_{21} & x_{23} k_{11} + x_{33} k_{21} \\
\end{bmatrix}
$$

Thus we get the derivatives

$$
\begin{align*}
\frac{ \partial y_{11} }{ \partial x_{11} } = k_{11} ~~&;~~
\frac{ \partial y_{11} }{ \partial x_{21} } = k_{21} \\

\frac{ \partial y_{12} }{ \partial x_{12} } = k_{11} ~~&;~~
\frac{ \partial y_{12} }{ \partial x_{22} } = k_{21} \\

\frac{ \partial y_{13} }{ \partial x_{13} } = k_{11} ~~&;~~
\frac{ \partial y_{13} }{ \partial x_{23} } = k_{21} \\

\frac{ \partial y_{21} }{ \partial x_{21} } = k_{11} ~~&;~~
\frac{ \partial y_{21} }{ \partial x_{31} } = k_{21} \\

\frac{ \partial y_{22} }{ \partial x_{22} } = k_{11} ~~&;~~
\frac{ \partial y_{22} }{ \partial x_{32} } = k_{21} \\

\frac{ \partial y_{23} }{ \partial x_{23} } = k_{11} ~~&;~~
\frac{ \partial y_{23} }{ \partial x_{33} } = k_{21} \\
\end{align*}
$$

And

$$
\begin{align*}
\frac{ \partial y_{11} }{ \partial k_{11} } = x_{11} ~~&;~~
\frac{ \partial y_{11} }{ \partial k_{21} } = x_{21} \\

\frac{ \partial y_{12} }{ \partial k_{11} } = x_{11} ~~&;~~
\frac{ \partial y_{12} }{ \partial k_{21} } = x_{22} \\

\frac{ \partial y_{13} }{ \partial k_{11} } = x_{13} ~~&;~~
\frac{ \partial y_{13} }{ \partial k_{21} } = x_{23} \\

\frac{ \partial y_{21} }{ \partial k_{11} } = x_{21} ~~&;~~
\frac{ \partial y_{21} }{ \partial k_{21} } = x_{31} \\

\frac{ \partial y_{22} }{ \partial k_{11} } = x_{22} ~~&;~~
\frac{ \partial y_{22} }{ \partial k_{21} } = x_{32} \\

\frac{ \partial y_{23} }{ \partial k_{11} } = x_{23} ~~&;~~
\frac{ \partial y_{23} }{ \partial k_{21} } = x_{33} \\
\end{align*}
$$

Missing partial $Y$ derivaties are implicitly $0$.

Now, by the chain rule

$$
    \frac{ \partial C }{ \partial k_{ij} } = \sum_{r,s = 1}^{2,3} \frac { \partial C }{ \partial y_{rs} } \frac{\partial y_{rs}}{\partial x_{ij}}
$$

$$
    \frac{ \partial C }{ \partial x_{ij} } = \sum_{r,s = 1}^{2,3} \frac { \partial C }{ \partial y_{rs} } \frac{\partial y_{rs}}{\partial x_{ij}}
$$ -->